theories/logrel/definition.v
@@ -1,6 +1,6 @@
 From main.prelude Require Import imports autosubst big_op_three.
 From main.surf_lang Require Import types.
-From main.dyn_lang Require Import definition lemmas lib.
+From main.dyn_lang Require Import definition lemmas lib labels.
 From main.logrel.lib Require Import weakestpre rfn.
 
 From iris.si_logic Require Export bi.
@@ -12,7 +12,6 @@ Section logrel.
   Context {ν : label} {Hν : NeverOccurs ν}.
 
   (* Definition pairs := list (prod label label). *)
-  Definition pairs := label -d> label -d> siProp.
 
   Definition unit_rel : val -d> val -d> siProp :=
     λ v v', (match v, v' with
@@ -45,15 +44,12 @@ Section logrel.
             | _, _ => False
             end)%I.
 
-  Inductive guarded := G_YesPlz | G_NoThanks.
+  (* Inductive guarded := G_YesPlz | G_NoThanks. *)
 
-  Definition arrow_rel (g : guarded) (Φ1 Φ2 : val -d> val -d> siProp) (L2 : label -d> label -d> siProp) :
+  Definition arrow_rel (F1 F2 : siProp -> siProp) (Φ1 Φ2 : val -d> val -d> siProp) (L2 : label -> label -> Prop) :
     val -d> val -d> siProp :=
     λ v v', (match v, v' with
-            | LamV e, LamV e' => (match g with
-                                | G_YesPlz => bi_later
-                                | G_NoThanks => id
-                                 end (∀ w w', Φ1 w w' -∗ ▷ rfn Φ2 L2 e.[of_val w/] e'.[of_val w'/]))
+            | LamV e, LamV e' => (F1 (∀ w w', Φ1 w w' -∗ F2 (rfn Φ2 L2 e.[of_val w/] e'.[of_val w'/])))
                   (* end) (∀ w w', ▷ Φ1 w w' -∗ rfn Φ2 L2 (AppAn (Lam e) (of_val w)) (AppAn (Lam e') (of_val w')))) *)
             | _, _ => False
             end)%I.
@@ -67,7 +63,8 @@ Section logrel.
             | LitV LitUnit, LitV LitUnit => unit_rel v v'
             | LitV (LitBool _), LitV (LitBool _) => bool_rel v v'
             | LitV (LitInt _), LitV (LitInt _) => int_rel v v'
-            | LamV _, LamV _ => (arrow_rel G_YesPlz Ψ Ψ Δ) v v'
+            | LamV _, LamV _ => (arrow_rel bi_later id Ψ Ψ Δ) v v'
+                                 (* only a later at the start to enforce contractiveness *)
             | InjLV _, InjLV _ => sum_rel (later_rfn Ψ) (later_rfn Ψ) v v'
             | InjRV _, InjRV _ => sum_rel (later_rfn Ψ) (later_rfn Ψ) v v'
             | PairV _ _, PairV _ _ => prod_rel (later_rfn Ψ) (later_rfn Ψ) v v'
@@ -95,7 +92,7 @@ Section logrel.
     by rewrite (fixpoint_unfold (valrel_unknown_pre Δ) v v').
   Qed.
 
-  Fixpoint valrel_typed (τ : type) : pairs -d> val -d> val -d> siProp :=
+  Fixpoint valrel_typed (τ : type) : (label → label → Prop) -d> val -d> val -d> siProp :=
     λ Δ v v', (
       match τ with
       | Base B => match B with
@@ -104,24 +101,25 @@ Section logrel.
                  | Int => int_rel v v'
                  end
       | Bin bin τ1 τ2 => match bin with
-                        | Arrow => arrow_rel G_NoThanks (valrel_typed τ1 Δ) (valrel_typed τ2 Δ) Δ v v'
+                        | Arrow => arrow_rel id id (valrel_typed τ1 Δ) (valrel_typed τ2 Δ) Δ v v'
+                                 (* only a later for the return expressions; such that they are equivalent to app; \x.e w ~ \x.e' w' *)
                         | Sum => sum_rel (valrel_typed τ1 Δ) (valrel_typed τ2 Δ) v v'
                         | Product => prod_rel (valrel_typed τ1 Δ) (valrel_typed τ2 Δ) v v'
                         end
       | Unknown => valrel_unknown Δ v v'
       end)%I.
 
-  Definition exprel_typed (τ : type) (Δ : pairs) : expr -d> expr -d> siProp :=
+  Definition exprel_typed (τ : type) (Δ : LabelRel) : expr -d> expr -d> siProp :=
     λ e e', rfn (valrel_typed τ Δ) Δ e e'.
 
-  Definition less_possibilities_then : relation pairs :=
-    fun Δ1 Δ2 => ∀ ℓ ℓ', Δ2 ℓ ℓ' -∗ Δ1 ℓ ℓ'.
+  (* Definition less_possibilities_then : relation LabelRel := *)
+  (*   fun Δ1 Δ2 => ∀ ℓ ℓ', Δ2 ℓ ℓ' -∗ Δ1 ℓ ℓ'. *)
 
-  Notation "a ⪯ b" := (less_possibilities_then a b) (at level 30).
+  (* Notation "a ⪯ b" := (less_possibilities_then a b) (at level 30). *)
 
-  Definition open_exprel_typed (Γ : list type) (e e' : expr) (R : pairs) (τ : type) :=
-    ∀ (Δ : pairs) (vs vs' : list val),
-        ⌜ R ⪯ Δ ⌝ ∗ big_sepL3 (fun τ v v' => valrel_typed τ Δ v v') Γ vs vs' ⊢
+  Definition open_exprel_typed (Γ : list type) (L : LabelRel) (e e' : expr) (τ : type) :=
+    ∀ (Δ : LabelRel) (H : le_permissive L Δ) (vs vs' : list val),
+        big_sepL3 (fun τ v v' => valrel_typed τ Δ v v') Γ vs vs' ⊢
             exprel_typed τ Δ e.[subst_list (of_val <$> vs)] e'.[subst_list (of_val <$> vs')].
 
 End logrel.
