theories/logrel/lib/rfn.v
@@ -1,5 +1,5 @@
 From main.prelude Require Import autosubst.
-From main.dyn_lang Require Import definition lemmas tactics.
+From main.dyn_lang Require Import definition lemmas tactics labels.
 From main.logrel.lib Require Import weakestpre.
 
 From iris.si_logic Require Export bi.
@@ -10,12 +10,14 @@ Section rfn.
   Definition val_lift_r : (val -d> val -d> siProp) -d> val -d> expr -d> siProp :=
     λ Φ v e', (∃ v', ⌜ rtc step_not_error e' (of_val v') ⌝ ∗ Φ v v')%I.
 
-  Definition lbl_lift_r : (label -d> label -d> siProp) -d> label -d> expr -d> siProp :=
-    λ L ℓ e', ((∃ t' ℓ', ⌜ rtc step_not_error e' t' ⌝ ∗ ⌜ faulty t' ℓ' ⌝ ∗ L ℓ ℓ')%I).
+  (* Definition lbl_lift_r : (label -> label -> Prop) -d> label -d> expr -d> siProp := *)
+  (* Definition lbl_lift_r : (label -d> label -d> iProp) -> label -> expr -> Prop := *)
+  Definition lbl_lift_r : (label -> label -> Prop) -> label -> expr -> Prop :=
+    λ L ℓ e', ((∃ t' ℓ', rtc step_not_error e' t' ∧ faulty t' ℓ' ∧ L ℓ ℓ')).
 
-  Definition rfn : (val -d> val -d> siProp) -d> (label -d> label -d> siProp) -d> expr -d> expr -d> siProp :=
+  Definition rfn : (val -d> val -d> siProp) -d> (label -> label -> Prop) -d> expr -d> expr -d> siProp :=
     λ Φ L e e', wp (λ v, val_lift_r Φ v e')%I
-                   (λ ℓ, lbl_lift_r L ℓ e')%I e.
+                   (λ ℓ, ⌜ lbl_lift_r L ℓ e' ⌝)%I e.
 
   (* Definition rfn : (val -d> val -d> siProp) -d> (label -d> label -d> siProp) -d> expr -d> expr -d> siProp := *)
   (*   λ Φ L e e', wp (λ v, ∃ v', ⌜ rtc step_not_error e' (of_val v') ⌝ ∗ Φ v v')%I *)
@@ -38,20 +40,23 @@ Section rfn.
       iExists w'. iFrame. admit. }
   Admitted.
 
-  Lemma rfn_impl e1 e2 Φ Φ' L L' :
-    ⊢ rfn Φ' L' e1 e2 -∗ (∀ ℓ ℓ', L' ℓ ℓ' -∗ L ℓ ℓ') -∗ (∀ v v', Φ' v v' -∗ Φ v v') -∗ rfn Φ L e1 e2.
+  Lemma rfn_impl e1 e2 Φ Φ' L L' (HLL' : le_permissive L' L) :
+    ⊢ rfn Φ' L' e1 e2 -∗ (∀ v v', Φ' v v' -∗ Φ v v') -∗ rfn Φ L e1 e2.
   Proof.
-    iIntros "He Hl Hv".
-    rewrite /rfn. iApply (wp_impl with "He [Hl]").
-    - iIntros (ℓ) "H". iDestruct "H" as (t' ℓ') "(Hs & Hf & HL)". iExists t', ℓ'. iFrame. by iApply "Hl".
+    iIntros "He Hv".
+    rewrite /rfn. iApply (wp_impl with "He").
+    - iIntros (ℓ) "%H". iPureIntro. destruct H as (t' & ℓ' & Hs & Hf & HL). exists t', ℓ'. naive_solver.
     - iIntros (v) "H". iDestruct "H" as (v') "(Hs & HΦ)". iExists v'. iFrame. by iApply "Hv".
   Qed.
 
   Lemma rfn_val v1 v2 e1 (H1 : e1 = of_val v1) e2 (H2 : e2 = of_val v2) Φ L : Φ v1 v2 ⊢ rfn Φ L e1 e2.
   Proof. rewrite /rfn. iIntros "HΦ". iApply wp_val. eauto. iExists v2. iFrame. iPureIntro. rewrite H2. by apply rtc_refl. Qed.
 
-  Lemma rfn_faulty e ℓ (H : faulty e ℓ) e' ℓ' (H' : faulty e' ℓ') Φ L : L ℓ ℓ' ⊢ rfn Φ L e e'.
-  Proof. iIntros "HΦ". rewrite /rfn /lbl_lift_r. iApply wp_faulty; eauto. Qed.
+  Lemma rfn_val_l_inv v1 e2 Φ L : rfn Φ L (of_val v1) e2 ⊢ val_lift_r Φ v1 e2.
+  Proof. rewrite /rfn. iIntros "H". by iDestruct (wp_val_inv with "H") as "H'". Qed.
+
+  Lemma rfn_faulty e ℓ (H : faulty e ℓ) e' ℓ' (H' : faulty e' ℓ') Φ L (HL : L ℓ ℓ') : ⊢ rfn Φ L e e'.
+  Proof. rewrite /rfn /lbl_lift_r. iApply wp_faulty; eauto. iPureIntro. eexists _, _; eauto. naive_solver. Qed.
 
   Instance rfn_proper : NonExpansive rfn.
   Proof. rewrite /rfn. intros n P P' dP L e e'. apply wp_proper. solve_proper. Qed.
@@ -60,7 +65,7 @@ Section rfn.
 
   Lemma rfn_impl_r {e e1} e2 Φ L
      (HΦ : ⊢ ∀ v, val_lift_r Φ v e2 -∗ val_lift_r Φ v e1)
-     (HL : ⊢ ∀ ℓ, lbl_lift_r L ℓ e2 -∗ lbl_lift_r L ℓ e1)
+     (HL : ∀ ℓ, lbl_lift_r L ℓ e2 → lbl_lift_r L ℓ e1)
     : ⊢ rfn Φ L e e2 -∗ rfn Φ L e e1.
   Proof. iIntros "H". iApply (wp_impl with "H"); eauto. Qed.
 
@@ -70,8 +75,8 @@ Section rfn.
     iApply rfn_impl_r.
     - iIntros (v) "H". iDestruct "H" as (v') "[%Hs Hv]". iExists v'. iFrame.
       iPureIntro. by eapply rtc_l.
-    - iIntros (v) "H". iDestruct "H" as (e' ℓ') "(%Hs & Hf & HL)".
-      rewrite /lbl_lift_r. iExists e', ℓ'. iFrame. iPureIntro. by eapply rtc_l.
+    - intros ℓ Hr. destruct Hr as (e' & ℓ' & Hs & Hf & HL).
+      rewrite /lbl_lift_r. exists e', ℓ'. split; auto. by eapply rtc_l.
   Qed.
 
   Lemma rfn_s_l {e1 e2} (H : step_not_error e1 e2) Φ L e' :
@@ -92,11 +97,11 @@ Section rfn.
         - simplify_eq. exfalso.
           assert (H' := step_no_val _ _ H). by rewrite to_of_val in H'.
         - simplify_eq. by rewrite (ne_step_det _ _ _ H H0). }
-    - iIntros (v) "H". rewrite /lbl_lift_r. iDestruct "H" as (e' ℓ') "(%Hs & %Hf & HL)".
+    - intros ℓ Hℓ. rewrite /lbl_lift_r. destruct Hℓ as (e' & ℓ' & Hs & Hf & HL).
       rewrite /lbl_lift_r.
       { inversion Hs; simplify_eq.
         - exfalso. by eapply faulty_not_stop.
-        - rewrite (ne_step_det _ _ _ H H0). iExists e', ℓ'. iSplit; auto. }
+        - rewrite (ne_step_det _ _ _ H H0). exists e', ℓ'. split; auto. }
   Qed.
 
   (* Lemma rfn_lam_app_later_body Φ L e e' w w' ν ν' : *)
