theories/logrel/lemmas/casts_compat.v
@@ -1,5 +1,5 @@
 From main.surf_lang Require Import types.
-From main.dyn_lang Require Import definition lib casts.
+From main.dyn_lang Require Import definition lib casts tactics.
 From main.prelude Require Import imports labels autosubst.
 
 From main.logrel Require Import definition.
@@ -12,7 +12,9 @@ Section casts_compat.
 
   Context {ν : label} {Hν : NeverOccurs ν}.
 
-  Lemma compat_cast_upwards_val L ℓ ℓ' (Hp : ⊢ L ℓ ℓ') (τ : type) :
+  Ltac rfn_faulty := (iApply rfn_faulty; [ by faulty_solver| by faulty_solver| auto ]).
+
+  Lemma compat_cast_upwards_val L ℓ ℓ' (HL : L ℓ ℓ') (τ : type) :
     ⊢ ∀ (dir : direction), match dir with
       | Normal =>
           (∀ v v', valrel_typed τ L v v' -∗
@@ -24,7 +26,6 @@ Section casts_compat.
                                       (AppAn (of_val $ cast_upwards ℓ' τ Opposite) (of_val v')))
     end.
   Proof.
-    iDestruct Hp as "#Hp".
     iInduction τ as [ B | const | asdf] "IH"; iIntros (dir).
     - destruct dir; simpl; iIntros (v v') "Hvv'".
       + rfn_steps. iNext. rfn_val.
@@ -47,8 +48,8 @@ Section casts_compat.
           [ iClear "IH"; iClear "IH1"; auto | repeat rewrite /= decide_False; auto ].
         * (* ? -> ? *)
           destruct dir; repeat rewrite /cast_upwards decide_True; auto; iIntros (v v') "#Hvv'".
-          { rfn_steps. rfn_val. rewrite /valrel_typed.
-            dvals v v'. rewrite valrel_unknown_unfold. auto. }
+          { rfn_steps. rfn_val. rewrite /arrow_rel.
+            dvals v v'. rewrite valrel_unknown_unfold /=. auto. }
           { rfn_steps. rfn_val. iNext.
             iIntros (w w') "#Hww'". rfn_steps.
             rewrite (valrel_unknown_unfold _ v v').
@@ -59,14 +60,13 @@ Section casts_compat.
         * destruct dir; repeat rewrite /cast_upwards decide_False; auto; iIntros (v v') "#Hvv'".
           { asimpl. rfn_steps. rfn_val.
             rewrite (valrel_unknown_unfold) /=. repeat iNext.
-            iIntros (w w') "#Hww'". asimpl. rfn_bind_pop'. by iApply "IH". iNext.
+            iIntros (w w') "#Hww'". asimpl. rfn_bind_pop'. by iApply "IH".
             iIntros (x x') "#Hxx'". dvals v v'; try rfn_faulty.
             rfn_steps. iSpecialize ("Hvv'" with "Hxx'"). iNext. rfn_bind'. by iApply "Hvv'". iApply "IH1". }
           { rfn_steps. rfn_val. rewrite (valrel_unknown_unfold) /=. iNext.
             iIntros (w w') "#Hww'". asimpl. rfn_bind_pop'. iApply ("IH" with "Hww'").
-            dvals v v'; try by (iNext; iIntros (y y') "Hyy'"; rfn_faulty).
-            iNext. iIntros (x x') "#Hxx'". iSpecialize ("Hvv'" with "Hxx'").
-            rfn_bind_pop'. rfn_steps. by iApply "Hvv'". iApply "IH1". }
+            iIntros (x x') "#Hxx'". dvals v v'; try rfn_faulty.
+            rfn_steps. iNext. iSpecialize ("Hvv'" with "Hxx'"). rfn_bind'. by iApply "Hvv'". iApply "IH1". }
       + (* sum case *)
         destruct (decide ((τ1 = Unknown) ∧ (τ2 = Unknown))) as [[-> ->] | bbb];
           [ repeat rewrite /= decide_True; auto | repeat rewrite /= decide_False; auto ].
@@ -107,7 +107,7 @@ Section casts_compat.
     - destruct dir; iIntros (v v') "Hvv'"; rfn_steps; rfn_val.
   Qed.
 
-  Lemma compat_cast_val (τ τ' : type) (H : consistency τ τ') L ℓ ℓ' (Hp : ⊢ L ℓ ℓ') :
+  Lemma compat_cast_val (τ τ' : type) (H : consistency τ τ') L ℓ ℓ' (HL : L ℓ ℓ')  :
     ⊢ ∀ (dir : direction), match dir with
       | Normal =>
           (∀ v v', valrel_typed τ L v v' -∗
@@ -119,12 +119,11 @@ Section casts_compat.
                                       (AppAn (of_val $ cast_pre ℓ' τ τ' H Opposite) (of_val v')))
     end.
   Proof.
-    iDestruct Hp as "Hp".
     iInduction H as [ τ | τ | B | bin τ1 τ1' τ2 τ2' H1 H2 ] "IH"; iIntros (dir).
     - by iApply compat_cast_upwards_val.
     - destruct dir.
-      + iApply (compat_cast_upwards_val _ _ _ Hp τ $! Opposite).
-      + iApply (compat_cast_upwards_val _ _ _ Hp τ $! Normal).
+      + iApply (compat_cast_upwards_val _ _ _ HL τ $! Opposite).
+      + iApply (compat_cast_upwards_val _ _ _ HL τ $! Normal).
     - destruct dir; iIntros (v v') "Hvv'"; rfn_steps;
         destruct B; dvals v v'; rfn_val.
     - destruct bin; iSpecialize ("IH1" $! dir);
@@ -133,10 +132,10 @@ Section casts_compat.
         | iSpecialize ("IH" $! dir) ].
       + destruct dir; rewrite /switch; iIntros (v v') "#Hvv'".
         * rfn_steps. rfn_val. iNext. iIntros (w w') "#Hww'". asimpl.
-          rfn_bind_pop'. by iApply "IH". iNext. iIntros (x x') "#Hxx'". dvals v v'. rfn_steps.
+          rfn_bind_pop'. by iApply "IH". iIntros (x x') "#Hxx'". dvals v v'. rfn_steps.
           iSpecialize ("Hvv'" with "Hxx'"). iNext. rfn_bind'. by iApply "Hvv'". iApply "IH1".
         * rfn_steps. rfn_val. iNext. iIntros (w w') "#Hww'". asimpl.
-          rfn_bind_pop'. by iApply "IH". iNext. iIntros (x x') "#Hxx'". dvals v v'. rfn_steps.
+          rfn_bind_pop'. by iApply "IH". iIntros (x x') "#Hxx'". dvals v v'. rfn_steps.
           iSpecialize ("Hvv'" with "Hxx'"). iNext. rfn_bind'. by iApply "Hvv'". iApply "IH1".
       + destruct dir; rewrite /switch; iIntros (v v') "#Hvv'".
         * rfn_steps. dvals v v'; try rfn_faulty; rfn_steps.
@@ -159,13 +158,13 @@ Section casts_compat.
           iIntros (x x') "Hxx'". rfn_val. iFrame.
   Qed.
 
-  Lemma compat_cast (τ τ' : type) (H : consistency τ τ') L ℓ ℓ' (Hp : ⊢ L ℓ ℓ') :
+  Lemma compat_cast (τ τ' : type) (H : consistency τ τ') L ℓ ℓ' (HL : L ℓ ℓ') :
     ⊢ (∀ e e', exprel_typed τ L e e' -∗
                       exprel_typed τ' L (AppAn (of_val $ cast ℓ τ τ' H) e)
                                         (AppAn (of_val $ cast ℓ' τ τ' H) e')).
   Proof.
     iIntros (e e') "Hee'". rfn_bind "Hee'".
-    by iDestruct (compat_cast_val _ _ H _ _ _ Hp $! Normal) as "H".
+    by iDestruct (compat_cast_val _ _ H _ _ _ HL $! Normal) as "H".
   Qed.
 
 End casts_compat.
