theories/logrel/lemmas/dyn_emb.v
@@ -1,7 +1,7 @@
 From main.prelude Require Import imports autosubst big_op_three.
 From main.surf_lang Require Import types.
-From main.dyn_lang Require Import definition lemmas.
-From main.logrel.lib Require Import weakestpre rfn.
+From main.dyn_lang Require Import definition lemmas tactics labels lib.
+From main.logrel.lib Require Import weakestpre rfn wrappers.
 
 From iris.si_logic Require Export bi.
 From iris.proofmode Require Import tactics.
@@ -13,23 +13,191 @@ Section fundamental_bare_rfn_demb.
 
   Context {ν : label} {Hν : NeverOccurs ν}.
 
-  Definition Δ (e : expr) : label -d> label -d> siProp.
-  Admitted.
+  Lemma rfn_bindK {K K' t t' e e' Ψ Φ L} :
+    t = fill K e →
+    t' = fill K' e' →
+    ⊢ rfn Ψ L e e' -∗ (∀ v v', Ψ v v' -∗ rfn Φ L (fill K (of_val v)) (fill K' (of_val v'))) -∗ rfn Φ L t t'.
+  Proof. intros. simplify_eq. iApply rfn_bind'. Qed.
 
-  Lemma cast_closed ℓ τ1 τ2 : Closed (of_val $ cast ℓ τ1 τ2).
-  Proof.
+  (* "bind pop left" *)
+  Ltac rfn_bind_pr :=
+    iApply rfn_bindK; [ simpl; by rw_fill; eauto | simpl; by rw_fill_popped; eauto | simpl | simpl ].
+
+  Ltac rfn_bind_pl :=
+    iApply rfn_bindK; [ simpl; by rw_fill_popped; eauto | simpl; by rw_fill; eauto | simpl | simpl ].
+
+  Ltac rfn_bind_pp :=
+    iApply rfn_bindK; [ simpl; by rw_fill_popped; eauto | simpl; by rw_fill_popped; eauto | simpl | simpl ].
+
+  Ltac rfn_bind :=
+    iApply rfn_bindK; [ simpl; by rw_fill; eauto | simpl; by rw_fill; eauto | simpl | simpl ].
+
+  Ltac permissive_solver :=
+      lazymatch goal with
+      | HΔ : le_permissive _ ?Δ |- le_permissive _ ?Δ =>
+          (apply (le_permissive_trans' _ _ _ HΔ), le_perm_unary_conj; intros k Hk; rewrite /occursIn; set_solver)
+      | _ => fail "ads"
+      end.
+
+ Lemma unary_conj_id H ℓ : H ℓ → unary_conj H ℓ ℓ.
+ Proof. intro. by split. Qed.
+
+    Ltac delta_solver :=
+      lazymatch goal with
+      | HΔ : le_permissive _ ?Δ |- ?Δ _ _ =>
+          (apply HΔ, unary_conj_id; rewrite /occursIn; set_solver)
+      | _ => fail "ads"
+      end.
 
 
-  Lemma emb_subst (e : expr) σ : ⌊ (⌜⌜ e ⌝⌝) ⌋.[σ] = ⌊ (⌜⌜ e.[σ] ⌝⌝) ⌋.
-  Proof.
-    induction e.
-    - rewrite 1 /dyn_emb. simpl.
+  Ltac rfn_faulty := (iApply rfn_faulty; [ by faulty_solver| by faulty_solver| by delta_solver ]).
+(*                      (iApply (rfn_faulty _ _ with "Hp"); faulty_solver). *)
 
-    (asimpl; naive_solver). try by naive_solver.
+
+
+  Ltac dvals v v' := destruct v, v'; repeat (lazymatch goal with | x : base_lit |- _ => destruct x end); auto.
+
+  Instance Ids_expr : Ids expr. derive. Defined.
+  Instance Var_Inj : Inj eq eq Var. intros x1 x2 eq. by inversion eq. Qed.
+
+Ltac closed_solver :=
+  lazymatch goal with
+  | H : Closed_n _ _ |- Closed_n _ _ => intros σ; specialize (H σ); simpl in H; by simplify_eq
+  | |- Closed_n _ _ => fail "goal detected suc"
+  | _ => fail "wrong goal"
+  end.
+
+
 
   Lemma fundamental_bare_rfn_demb (e : expr) n (Hne : Closed_n n e) :
-    open_exprel_typed (replicate n Unknown) e  (⌊ (⌜⌜ e ⌝⌝) ⌋) (Δ e) Unknown.
+    open_exprel_typed (replicate n Unknown) (Lbls e) e (⌊ (⌜⌜ e ⌝⌝) ⌋) Unknown.
   Proof.
+    generalize dependent n.
+    induction e; iIntros (n Hn Δ HΔ vs vs') "#Hvsvs'".
+    - admit.
+    - admit.
+    - rfn_bind. iApply (IHe1 n with "Hvsvs'"). { intros σ. specialize (Hn σ). inversion Hn. by repeat rewrite H0.  } permissive_solver.
+      iIntros (v v') "#Hvv'". simpl. rfn_steps.
+      rewrite valrel_unknown_unfold. dvals v v'; try by rfn_faulty.
+      iRewrite "Hvv'". destruct b0; rfn_steps; iNext.
+      iApply (IHe2 n ltac:(closed_solver) Δ ltac:(permissive_solver) with "Hvsvs'").
+      iApply (IHe3 n ltac:(closed_solver) Δ ltac:(permissive_solver) with "Hvsvs'").
+    - rfn_bind.
+      iApply (IHe1 n ltac:(closed_solver) Δ ltac:(permissive_solver) with "Hvsvs'").
+      iIntros (v1 v1') "#H1". asimpl.
+      rfn_bind.
+      iApply (IHe2 n ltac:(closed_solver) Δ ltac:(permissive_solver) with "Hvsvs'").
+      iIntros (v2 v2') "#H2".
+      rfn_steps.
+      do 2 rewrite valrel_unknown_unfold. dvals v1 v1'; try by rfn_faulty.
+      dvals v2 v2'; rfn_steps; try by rfn_faulty. rfn_val. iRewrite "H1". iRewrite "H2". do 2 rewrite Z.add_0_l.
+      rewrite valrel_unknown_unfold; destruct binop; auto.
+    - assert (Hlt := (iffLR (ids_lt_Closed_n _ _) Hn)). iDestruct ((big_sepL3_length _ (replicate n Unknown) vs vs' with "Hvsvs'")) as "[%eq %eq']".
+      destruct (lookup_lt_is_Some_2 (replicate n Unknown) v) as [τ Hτ].
+      rewrite replicate_length. lia. rewrite replicate_length in eq. simplify_eq.
+      destruct (ids_subst_list_lt_length (v) (of_val <$> vs)) as (w1 & eq1 & eq1'). by rewrite map_length.
+      destruct (ids_subst_list_lt_length (v) (of_val <$> vs')) as (w2 & eq2 & eq2'). rewrite map_length. lia.
+      asimpl in *. rewrite eq1' eq2'. clear eq1' eq2'.
+      destruct (list_lookup_fmap_inv _ _ _ _ eq1) as (a1 & eq1' & eq1'').
+      destruct (list_lookup_fmap_inv _ _ _ _ eq2) as (a2 & eq2' & eq2'').
+      simplify_eq. rfn_val. iApply (big_sepL3_lookup with "Hvsvs'"); eauto. apply lookup_replicate. split; auto.
+    - asimpl. rewrite decide_True; auto. rfn_steps. rfn_val. rewrite valrel_unknown_unfold.
+      simpl. iNext. iIntros (w w') "Hww'". asimpl. iNext.
+      replace e.[of_val w .: subst_list (of_val <$> vs)] with e.[subst_list ((of_val w) :: (of_val <$> vs))] by by asimpl.
+      replace (⌊ ⌜⌜ e ⌝⌝ ⌋).[of_val w' .: subst_list (of_val <$> vs')] with (⌊ ⌜⌜ e ⌝⌝ ⌋).[subst_list ((of_val w') :: (of_val <$> vs'))] by by asimpl.
+      do 2 rewrite -fmap_cons.
+      iApply (IHe (S n) ltac:(closed_solver) Δ ltac:(permissive_solver)). simpl. auto.
+    - asimpl. rewrite decide_True; auto. rfn_steps.
+      rfn_bind.
+      iApply (IHe1 n ltac:(closed_solver) Δ ltac:(permissive_solver) with "Hvsvs'").
+      iIntros (v1 v1') "#H1". asimpl.
+      rfn_steps.
+      rfn_bind.
+      iApply (IHe2 n ltac:(closed_solver) Δ ltac:(permissive_solver) with "Hvsvs'").
+      iIntros (v2 v2') "#H2". asimpl.
+      rfn_steps.
+      rewrite valrel_unknown_unfold. dvals v1 v1'; try by rfn_faulty.
+      rewrite /valrel_unknown_pre /arrow_rel.
+      rfn_steps. iNext.
+      iNext.
+
+
+      rfn_bind_pl.
+
+
+      iApply rfn_s_r.
+      rw_of_val.
+      change (App ?ℓ (of_val ?v) ?e) with (fill_item (AppRCtx ℓ v) e).
+      change (App ?ℓ (of_val ?v) ?e) with (fill_item (AppRCtx ℓ v) e).
+      change (App ?ℓ (of_val ?v) ?e) with (fill_item (AppRCtx ℓ v) e).
+      change (App ?ℓ (of_val ?v) ?e) with (fill_item (AppRCtx ℓ v) e).
+      rw_fill_popped.
+      eapply stepK. eauto. simpl.
+      econstructor.
+
+
+
+      rw_fill_item. rw_fill.
+      rw_fill_popped.
+      eapply stepK. eauto. simpl.
+   change (fill_item ?Ki1 (fill_item ?Ki2 ?e))
+     with (fill [Ki1; Ki2] e).
+
+   change (fill_item ?Ki1 (fill_item ?Ki2 (fill_item ?Ki3 ?e)))
+          (fill [Ki1] (fill_item ?Ki2 (fill_item ?Ki3 ?e))).
+     with (fill [Ki1 ; Ki2] (fill_item Ki3 e)).
+
+
+      iApply rfn_bindK. rw_fill_item.
+      change (App ?ℓ ?e1 ?e2) with (fill_item (AppLCtx ℓ e2) e1).
+
+      iApply rfn_bindK; [ simpl; by rw_fill; eauto | simpl; by rw_fill_popped; eauto | simpl | simpl ].
+
+      rfn_bind_pr.
+
+    iApply (IHe (S n) ltac:(closed_solver) Δ ltac:(permissive_solver)). simpl. auto.
+    -
+
+
+
+
+
+
+Ltac rfn_faulty := by (iApply (rfn_faulty _ _ with "Hp"); faulty_solver).
+
+      lazymatch goal with
+      | HΔ : le_permissive _ Δ |- le_permissive _ Δ =>
+          (apply (le_permissive_trans' _ _ _ HΔ), le_perm_unary_conj; intros k Hk; rewrite /occursIn; set_solver)
+      | _ => fail "ads"
+      end.
+
+
+
+      assert (Hc1 : Closed_n n e1). admit.
+      assert (Hl1 : le_permissive (Lbls e1) Δ).
+
+      iDestruct (IHe1 _ Hc1 Δ Hl1 vs vs' with "Hvsvs'") as "HH".
+      simpl.
+
+       iApply rfn_bindK. simpl. rw_fill; eauto. rw_fill_popped; eauto. simpl.
+      iApply ("IH" $! n). admit. iFrame "Hvsvs'". iPureIntro.
+
+
+      iSpecialize
+
+    - admit.
+    - admit.
+    - admit.
+
+
+
+
+
+
+
+
+
+
     generalize dependent n.
     iInduction e as
       [ (* Lit *) b | (* Seq *) ℓ e1 e2 | (*If*) ℓ e0 e1 e2
@@ -37,8 +205,29 @@ Section fundamental_bare_rfn_demb.
       | (* App *) ℓ e1 e2 | (* InjL *) e | (* InjR *) e
       | (* Case *) ℓ e e1 e2 | (* Fst *) ℓ e | (* Snd *) ℓ e
       | (* Pair *) e1 e2 | (* Error *) ℓ] "IH";
-      iIntros (n Hn P vs vs') "[%Hlp Hvsvs']".
-    - admit.
+      iIntros (n Hn P vs vs') "[%Hlp #Hvsvs']".
+    - rfn_steps. rfn_val. rewrite valrel_unknown_unfold /=. destruct b; auto.
+    - rfn_bind. iApply ("IH" $! n). admit. iFrame "Hvsvs'".
+      iPureIntro.
+
+      Δ(Seq ℓ e1 e3) ≤ P, then Δ e1 ≤ P
+      in general, if P
+
+    - asimpl.
+
+      (* rfn_bind_pr. *)
+      iApply rfn_bindK. rw_fill; eauto. rw_fill_popped; eauto. simpl.
+      iApply ("IH" $! n). admit. iFrame "Hvsvs'". iPureIntro.
+
+
+
+
+      intros        cha
+      rfn_bind
+
+      rfn_steps. rfn_val. rewrite valrel_unknown_unfold /=. destruct b; auto.
+
+
     - asimpl. admit.
     - asimpl. iSpecialize ("IH" $! n ).
       (* specialize with P, *)
